TypedAssembly/LambdaF/TermEnv.lean
@@ -17,12 +17,27 @@ inductive Lookup : Ctx Δ → Δ ⊢F⋆ ⋆ → Type where
   | there {Γ : Ctx Δ} {t₁ t₂ : Δ ⊢F⋆ ⋆} : Lookup Γ t₁ → Lookup (Γ ,, t₂) t₁
   | move  {Γ : Ctx Δ} {t : Δ ⊢F⋆ ⋆} {k} : Lookup Γ t →
                                           Lookup (Γ ,,⋆ k) (weakenτ t)
-deriving Repr
 
 namespace Lookup
   infix:40 " ∋ " => Lookup
+
+  def toNat : Γ ∋ t → Nat × Nat
+    | .here => (0, 0)
+    | .there x => 
+      let (n, m) := x.toNat 
+      (n + 1, m)
+    | .move x => 
+      let (n, m) := x.toNat 
+      (n, m + 1)
+
+  def repr (x : Γ ∋ t) : String :=
+    let (n, m) := x.toNat
+    s!"#{m.repeat (· ++ "⊹") ""}{n}"
 end Lookup
 open Lookup
+
+instance : Repr (Γ ∋ t) where
+  reprPrec x _ := x.repr
 
 def conv_ni {Δ Γ} {t₁ t₂ : Δ ⊢F⋆ ⋆} : t₁ = t₂ → (Γ ∋ t₁) → Γ ∋ t₂
   | rfl, a => a
